code/streaming/Hacl.Streaming.Functor.fsti
@@ -1,0 +1,285 @@
+module Hacl.Streaming.Functor
+
+/// Provided an instance of the type class, this creates a streaming API on top.
+/// This means that every function in this module takes two extra arguments
+/// compared to the previous streaming module specialized for hashes: the type
+/// of the index, and a type class for that index. Then, as usual, a given value
+/// for the index as a parameter.
+
+#set-options "--max_fuel 0 --max_ifuel 0"
+
+module ST = FStar.HyperStack.ST
+module HS = FStar.HyperStack
+module B = LowStar.Buffer
+module G = FStar.Ghost
+module S = FStar.Seq
+module U32 = FStar.UInt32
+module U64 = FStar.UInt64
+
+open Hacl.Streaming.Interface
+open FStar.HyperStack.ST
+open LowStar.BufferOps
+open FStar.Mul
+
+inline_for_extraction noextract
+let uint8 = Lib.IntTypes.uint8
+
+inline_for_extraction noextract
+let uint32 = Lib.IntTypes.uint32
+
+/// State machinery
+/// ===============
+
+[@CAbstractStruct]
+val state_s (#index: Type0) (c: block index) (i: index): Type0
+
+let state #index (c: block index) (i: index) = B.pointer (state_s c i)
+
+val freeable (#index: Type0) (c: block index) (i: index) (h: HS.mem) (p: state c i): Type0
+
+let preserves_freeable #index (c: block index) (i: index) (s: state c i) (h0 h1: HS.mem): Type0 =
+  freeable c i h0 s ==> freeable c i h1 s
+
+val footprint_s (#index: Type0) (c: block index) (i: index) (h: HS.mem) (s: state_s c i): GTot B.loc
+
+let footprint (#index: Type0) (c: block index) (i: index) (m: HS.mem) (s: state c i) =
+  B.(loc_union (loc_addr_of_buffer s) (footprint_s c i m (B.deref m s)))
+
+/// Invariants
+/// ==========
+
+noextract
+let bytes = S.seq uint8
+
+let loc_includes_union_l_footprint_s
+  #index
+  (c: block index)
+  (i: index)
+  (m: HS.mem)
+  (l1 l2: B.loc) (s: state_s c i)
+: Lemma
+  (requires (
+    B.loc_includes l1 (footprint_s c i m s) \/ B.loc_includes l2 (footprint_s c i m s)
+  ))
+  (ensures (B.loc_includes (B.loc_union l1 l2) (footprint_s c i m s)))
+  [SMTPat (B.loc_includes (B.loc_union l1 l2) (footprint_s c i m s))]
+= B.loc_includes_union_l l1 l2 (footprint_s c i m s)
+
+val invariant_s (#index: Type0) (c: block index) (i: index) (h: HS.mem) (s: state_s c i): Type0
+
+let invariant #index (c: block index) (i: index) (m: HS.mem) (s: state c i) =
+  B.live m s /\
+  B.(loc_disjoint (loc_addr_of_buffer s) (footprint_s c i m (B.deref m s))) /\
+  invariant_s c i m (B.get m s 0)
+
+val invariant_loc_in_footprint
+  (#index: Type0)
+  (c: block index)
+  (i: index)
+  (s: state c i)
+  (m: HS.mem)
+: Lemma
+  (requires (invariant c i m s))
+  (ensures (B.loc_in (footprint c i m s) m))
+  [SMTPat (invariant c i m s)]
+
+/// Keeping track of the bytes fed into the algorithm so far
+/// ========================================================
+///
+/// We offer a stateful predicate that allows the client to tie a particular
+/// state to a sequence of bytes hashed so far. There are a variety of styles
+/// possible, here's a recap and a discussion of the respective merits of each
+/// style, so that we document and avoid going back and forth for future APIs.
+///
+/// 1. val update (b: erased bytes): unit
+///      requires (fun h0 -> hashes h0 s b)
+///      ensures (fun h1 -> hashes h1 s (b `append` data))
+///
+///    The problem with this one is that it requires the client to not only
+///    explicitly pass an erased argument, but also requires the client, when
+///    chaining calls to construct the "next" value by manually concatenating
+///    (ghostly) bytes.
+///
+/// 2. val update (b: erased bytes): erased bytes
+///      requires (fun h0 -> hashes h0 s b)
+///      ensures (fun h1 b' -> hashes h1 s b' /\ b' == b `append` data)
+///
+///    This one is a slight improvement over 1. because the client can "get
+///    their hands" on the returned bytes and doesn't need to manually create
+///    the concatenation ``b `append` data`` when they chain another call to
+///    update.
+///
+/// 3. val update (): unit
+///      requires _
+///      ensures (fun h0 _ h1 -> hashed h1 s == hashed h0 s `append` data)
+///
+///    While 1. and 2. were based on a predicate, this one relies on a function
+///    that returns the bytes (ghostly) for any given state and heap. It does
+///    not require the client to materialize the erased bytes, and it does not
+///    require the client to manually construct intermediary ghost byte values
+///    when chaining.
+///
+/// 4. There's another style based on a state machine and an erased value that
+///    materializes all the ghost state in a single record, thus requiring only a
+///    single framing lemma (as opposed to three or more for the styles 1. 2. and
+///    3.). It appears that this may be overkill for this module and may be better
+///    suited to TLS.
+///
+///                                            JP (20190607)
+
+val seen: #index:Type0 -> c:block index -> i:index -> h:HS.mem -> s:state c i -> GTot bytes
+
+/// Framing
+/// =======
+///
+/// Everything a client needs to know when they modify something **disjoint**
+/// from a hash state.
+///
+/// Note that the invariant now bundles a variety of conditions related to the
+/// hashing predicate, meaning that the only way to establish the invariant is
+/// actually to initialize the underlying state. This means that the framing
+/// lemmas for invariant and hashed could be bundled together. If we committed
+/// to always heap allocating, then we could conceivably have a single framing
+/// lemma.
+
+val frame_invariant: #index:Type0 -> c:block index -> i:index -> l:B.loc -> s:state c i -> h0:HS.mem -> h1:HS.mem -> Lemma
+  (requires (
+    invariant c i h0 s /\
+    B.loc_disjoint l (footprint c i h0 s) /\
+    B.modifies l h0 h1))
+  (ensures (
+    invariant c i h1 s /\
+    footprint c i h0 s == footprint c i h1 s))
+  [ SMTPat (invariant c i h1 s); SMTPat (B.modifies l h0 h1) ]
+
+val frame_seen: #index:Type0 -> c:block index -> i:index -> l:B.loc -> s:state c i -> h0:HS.mem -> h1:HS.mem -> Lemma
+  (requires (
+    invariant c i h0 s /\
+    B.loc_disjoint l (footprint c i h0 s) /\
+    B.modifies l h0 h1))
+  (ensures (seen c i h0 s == seen c i h1 s))
+  [ SMTPat (seen c i h1 s); SMTPat (B.modifies l h0 h1) ]
+
+val frame_freeable: #index:Type0 -> c:block index -> i:index -> l:B.loc -> s:state c i -> h0:HS.mem -> h1:HS.mem -> Lemma
+  (requires (
+    invariant c i h0 s /\
+    freeable c i h0 s /\
+    B.loc_disjoint l (footprint c i h0 s) /\
+    B.modifies l h0 h1))
+  (ensures (freeable c i h1 s))
+  [ SMTPat (freeable c i h1 s); SMTPat (B.modifies l h0 h1) ]
+
+
+/// Stateful API
+/// ============
+
+val create_in (#index: Type0) (c: block index) (i: index) (r: HS.rid): ST (state c i)
+  (requires (fun _ ->
+    HyperStack.ST.is_eternal_region r))
+  (ensures (fun h0 s h1 ->
+    invariant c i h1 s /\
+    seen c i h1 s == S.empty /\
+    B.(modifies loc_none h0 h1) /\
+    B.fresh_loc (footprint c i h1 s) h0 h1 /\
+    B.(loc_includes (loc_region_only true r) (footprint c i h1 s)) /\
+    freeable c i h1 s))
+
+val init: #index:Type0 -> c:block index -> i:G.erased index -> (
+  let i = G.reveal i in
+  s:state c i -> Stack unit
+  (requires (fun h0 ->
+    invariant c i h0 s))
+  (ensures (fun h0 _ h1 ->
+    preserves_freeable c i s h0 h1 /\
+    invariant c i h1 s /\
+    seen c i h1 s == S.empty /\
+    footprint c i h0 s == footprint c i h1 s /\
+    B.(modifies (footprint c i h0 s) h0 h1))))
+
+unfold
+let update_pre
+  #index
+  (c: block index)
+  (i: index)
+  (s: state c i)
+  (data: B.buffer uint8)
+  (len: UInt32.t)
+  (h0: HS.mem)
+=
+  invariant c i h0 s /\
+  B.live h0 data /\
+  U32.v len = B.length data /\
+  S.length (seen c i h0 s) + U32.v len < c.max_input_length i /\
+  B.(loc_disjoint (loc_buffer data) (footprint c i h0 s))
+
+unfold
+let update_post
+  #index
+  (c: block index)
+  (i: index)
+  (s: state c i)
+  (data: B.buffer uint8)
+  (len: UInt32.t)
+  (h0 h1: HS.mem)
+=
+  preserves_freeable c i s h0 h1 /\
+  invariant c i h1 s /\
+  B.(modifies (footprint c i h0 s) h0 h1) /\
+  footprint c i h0 s == footprint c i h1 s /\
+  seen c i h1 s == seen c i h0 s `S.append` B.as_seq h0 data
+
+val update:
+  #index:Type0 ->
+  c:block index ->
+  i:G.erased index -> (
+  let i = G.reveal i in
+  s:state c i ->
+  data: B.buffer uint8 ->
+  len: UInt32.t ->
+  Stack unit
+    (requires fun h0 -> update_pre c i s data len h0)
+    (ensures fun h0 s' h1 -> update_post c i s data len h0 h1))
+
+/// A word of caution. Once partially applied to a type class, this function
+/// will generate a stack allocation at type ``state i`` via ``c.alloca``. If
+/// ``state`` is indexed over ``i``, then this function will not compile to C.
+/// (In other words: there's a reason why mk_finish does *NOT* take i ghostly.)
+///
+/// To work around this, it suffices to apply ``mk_finish`` to each possible
+/// value for the index, then to abstract over ``i`` again if agility is
+/// desired. See EverCrypt.Hash.Incremental for an example. Alternatively, we
+/// could provide a finish that relies on a heap allocation of abstract state
+/// and does not need to be specialized.
+inline_for_extraction noextract
+val mk_finish:
+  #index:Type0 ->
+  c:block index ->
+  i:index ->
+  s:state c i ->
+  dst:B.buffer uint8 { B.len dst == c.output_len i } ->
+  Stack unit
+    (requires fun h0 ->
+      invariant c i h0 s /\
+      B.live h0 dst /\
+      B.(loc_disjoint (loc_buffer dst) (footprint c i h0 s)))
+    (ensures fun h0 s' h1 ->
+      preserves_freeable c i s h0 h1 /\
+      invariant c i h1 s /\
+      seen c i h0 s == seen c i h1 s /\
+      footprint c i h0 s == footprint c i h1 s /\
+      B.(modifies (loc_union (loc_buffer dst) (footprint c i h0 s)) h0 h1) /\
+      S.length (seen c i h0 s) <= c.max_input_length i /\
+      S.equal (B.as_seq h1 dst) (c.spec_s i (seen c i h0 s)))
+
+val free:
+  #index:Type0 ->
+  c:block index ->
+  i:G.erased index -> (
+  let i = G.reveal i in
+  s:state c i ->
+  ST unit
+  (requires fun h0 ->
+    freeable c i h0 s /\
+    invariant c i h0 s)
+  (ensures fun h0 _ h1 ->
+    B.modifies (footprint c i h0 s) h0 h1))
